\title{SAGA - bound on function values}
\author{Aurelien Lucchi, Hadi Daneshmand, Thomas Hofmann}

\documentclass[12pt]{article}

\usepackage{amsmath,amssymb,amsthm}
\usepackage{booktabs}  % used for nice looking tables
\usepackage{graphicx}
\usepackage{hyperref}
\usepackage[margin=0.5in]{geometry}

\newcommand{\comment}[1]{}

\newcommand{\g}{{\bf g}}
\newcommand{\vectornorm}[1]{\left|\left|#1\right|\right|}
\newcommand{\sqnorm}[1]{\left|\left|#1\right|\right|^2} 
\newcommand{\w}{{\bf w}}
\newcommand{\wstar}{{\bf w^*}}
\newcommand{\wt}{{\bf w_t}}
\newcommand{\wT}{{\bf w_T}}
\newcommand{\wavg}{{\bf \bar{w}_T}}
\newcommand{\wavgn}{{\bf \bar{w}_n}}
\newcommand{\wavgb}{{\bf \bar{w}_T^{\prime}}}
\newcommand{\wsuffixavg}{{\bf \bar{w}_T^{\alpha}}}
\newcommand{\h}{{\bf h}}
\renewcommand{\u}{{\bf u}}
\newcommand{\x}{{\bf x}}
\newcommand{\xstar}{{\bf x^*}}
\newcommand{\y}{{\bf y}}
\newcommand{\z}{{\bf z}}
\newcommand{\E}{\mathbb{E}}
\newcommand{\R}{{\mathcal R}}
\newcommand*\diff{\mathop{}\!\mathrm{d}}
\renewcommand{\L}{{\mathcal L}}
\newcommand{\Hbar}{\bar{H}}

\newtheorem{theorem}{Theorem}
\newtheorem{lemma}[theorem]{Lemma}
\newtheorem{proposition}[theorem]{Proposition}
\newtheorem{corollary}[theorem]{Corollary}

\begin{document}
\maketitle

\noindent Lipschitz continuous gradients (upper quadratic bound), unbiasedness 
\begin{align}
& f(\w) - \E f(\w^{+}) \ge  \eta \| \nabla f(\w) \|^2  - \frac{\eta^2  L }{2}\E  \| g_i\|^2
\end{align}
One can exploit strong convexity to further bound the first term on the RHS
\begin{align}
\| \nabla f(\w) \|^2 \le 2 \mu \delta f(\w) 
\end{align}
Moreover 
\begin{align}
\E \| g_i(\w)\|^2 \leq 4L  \delta f(\w)  + 2 \E \|\alpha_i - \nabla f_i(\wstar)\|^2
\end{align}
So that one gets 
\begin{align}
\E \delta f(\w^{+})  \le \left( 1 - 2 \eta \mu + 4 \eta^2 L \right) \delta f(\w^{}) + 2 \E \|\alpha_i - \nabla f_i(\wstar)\|^2
\end{align}
If the variance correction was optimal, the last term would vanish and 
\begin{align}
\max_\eta \underbrace{\left\{  1-2\mu \eta + 4 \eta^2 L \right\}}_{\rho(\eta)} \iff \eta^* = \frac{ \mu }{4L} 
\Longrightarrow \rho^* =  1 - \frac{\mu^2}{2L} + \frac{\mu^2}{4L} = 1 - \frac{\mu^2}{4L}
\end{align}
Even in the simple analysis, we get an additional factor $\mu$ that is not good!

\noindent Compare this to the original proof 
\begin{align}
  \E \| \delta \w^+ \|^2 \le (1- \eta \mu) \| \delta \w\|^2 + (2\eta - 4\eta^2L) \delta f(\w) - 2 \eta^2 \E\|...\|^2
\end{align}
If now again, we ignore the last term and bound suboptimality via 
\begin{align}
\delta f(\w) \le \frac L2 \| \delta \w\|^2
\end{align}
so that we get 
\begin{align}
  \E \| \delta \w^+ \|^2 \le (1- \eta \mu) \| \delta \w\|^2 + (\eta L - 2\eta^2 L^2) \| \delta \w\|^2 - 2 \eta^2 \E\|...\|^2
\end{align}
and thus 
\begin{align}
\eta^* =  \frac{1-\frac \mu L }{4 L}
\end{align}
We can also approximate this by dropping the $-\mu$ term and get in essence 
\begin{align}
\eta = 
\end{align}

\newpage



\paragraph{Assumptions} Consider $f$ to be $\mu$-strongly-convex and differentiable with L-Lipschitz-continuous gradients, then $\forall \w \in \mathbb{R}^d$,
\begin{equation}
\sqnorm{\w - \wstar} \leq \frac{2}{\mu} \left( f(\w) - f(\wstar) \right)
\end{equation}

\begin{equation}
\sqnorm{\nabla f(\w)} \geq 2 \mu ( f(\w) - f(\wstar) )
\label{eq:strong_convex}
\end{equation}

%\begin{equation}
%f(\w) - f(\wstar) \leq \frac{L}{2} \sqnorm{\w - \wstar}
%\end{equation}

\begin{equation}
f(\w) \leq f(\w') + (\w-\w')^T \nabla f(\w') + \frac{L}{2} \sqnorm{\w-\w'} \;\; \forall \w' \in \mathbb{R}^d
\label{eq:smooth}
\end{equation}

\begin{equation}
\E \sqnorm{\nabla f_i(\w) - \nabla f_i(\wstar)} \leq 2L (f(\w) - f(\wstar))
\label{eq:bound_variance_f}
\end{equation}

\paragraph{SAGA}

We here the following SAGA update:
\begin{equation}
\w_{t+1} = \w_t - \eta g_i(\w_t),
\end{equation}
where $g_i(\w) = \nabla f_i(\w) - \alpha_i + \E_i \alpha_i $.\\

We start by proving two lemmas that will be used to establish the desired bound.

\begin{lemma}
\label{lemma:bound_f}
\begin{equation}
f(\w_{t+1}) \leq f(\w_t) - \eta \sqnorm{\nabla f(\w_t)} + \frac{\eta^2 L}{2} \E \sqnorm{g_i(\w_t)}
\label{eq:bound_f}
\end{equation}
\end{lemma}
\begin{proof}

Using $\w = \w_{t+1}$ and $\w' = \w_t$ in Eq.~\ref{eq:smooth}, we get:
\begin{equation}
f(\w_{t+1}) \leq f(\w_t) - \eta \nabla g_i(\w_t)^T \nabla f(\w_t) + \frac{\eta^2 L}{2} \sqnorm{g_i(\w_t)}
\end{equation}

Taking the expectation over $i$ concludes the proof.
\end{proof}

\begin{lemma}
\begin{align}
\sqnorm{g_i(\w)} \leq (1+\beta) \E \sqnorm{\nabla f_i(\w) - \nabla f_i(\wstar)} + (1+\beta^{-1}) \E \sqnorm{\alpha_i - \nabla f_i(\wstar)}
\label{eq:bound_variance}
\end{align}
\end{lemma}
\begin{proof}
See nSAGA.
\end{proof}

\begin{lemma}
Let $\delta f(\w_{t+1}) := f(\w_{t+1}) - f(\wstar)$. Then
\begin{align}
\delta f(\w_{t+1})
&\leq \delta f(\w_{t}) + \left( L^2 \eta^2 (1+\beta) - \eta \mu \right) \delta f(\w_{t})
+ \frac{L}{2} \eta^2 (1+\beta^{-1}) \E \sqnorm{\alpha_i - \nabla f_i(\wstar)}
\label{eq:bound_f}
\end{align}
\end{lemma}
\begin{proof}
Starting from Lemma~\ref{lemma:bound_f}
\begin{align}
\delta f(\w_{t+1})
&\leq \delta f(\w_{t}) - \eta \sqnorm{\nabla f(\w_t)} + \frac{L}{2} \eta^2 \E \sqnorm{g_i(\w_t)} \nonumber \\
&\stackrel{Eq.~\ref{eq:bound_variance}}\leq \delta f(\w_{t}) - \eta \sqnorm{\nabla f(\w_t)} + \frac{L}{2} \eta^2 ((1+\beta) \E \sqnorm{\nabla f_i(\w_t) - \nabla f_i(\wstar)} \nonumber \\
&+ (1+\beta^{-1}) \E \sqnorm{\alpha_i - \nabla f_i(\wstar)}) \nonumber \\
&\stackrel{Eq.~\ref{eq:bound_variance_f}}\leq \delta f(\w_{t}) + \left( L^2 \eta^2 (1+\beta) - \eta \mu \right) \delta f(\w_{t})
+ \frac{L}{2} \eta^2 (1+\beta^{-1}) \E \sqnorm{\alpha_i - \nabla f_i(\wstar)}
\end{align}

\end{proof}

Recall $\E \sqnorm{\alpha_i - \nabla f_i(\wstar)} \leq \Hbar$ (see nSAGA). We define the following Lyapnunov function
\begin{align}
\L(\w, H) := \delta f(\w) + S\alpha \Hbar.
\end{align}

\begin{theorem}
For $c \in (0; 1]$ and $\alpha \in [0;1]$, the following bound holds
\begin{equation}
\L(\w_{t+1}, H_{t+1}) \leq (1-\rho) \L(\w_t, H_t), \rho := c \eta \mu
\end{equation}

\end{theorem}

\begin{proof}

First note that $\E \Hbar_{t+1} = \left(\frac{n-1}{n} \Hbar_t + \frac{2L}{n} \delta f(\w_t) \right)$. Combining this equality with Eq.~\ref{eq:bound_f}, we get the following bound on $\Delta := \L(\w_{t+1}, H_{t+1}) - \L(\w_t, H_t)$:

\begin{align}
\Delta &\leq
\left( L^2 \eta^2 (1+\beta) - \eta \mu \right) \delta f(\w_{t}) + \frac{L}{2} \eta^2 (1+\beta^{-1}) \E \sqnorm{\alpha_i - \nabla f_i(\wstar)} \nonumber \\
&+ S\alpha \left( - \frac{1}{n} \Hbar + \frac{2L}{n} \delta f(\w_t) \right) \nonumber \\
&= \left[ L^2 \eta^2 (1+\beta) - \eta \mu \right] \delta f(\w_{t}) + \left[ \frac{L}{2} \eta^2 (1+\beta^{-1}) - \frac{S\alpha}{n} \right] \Hbar + \left[ \frac{2LS \alpha}{n} \right] \delta f(\w_t)
\end{align}

We now check under what conditions $\Delta := \L(\w_{t+1}, H_{t+1}) - \L(\w_t, H_t) \leq -\rho \L(\w_t, H_t)$

We start with the terms in the first and last rectangular brackets. Recall that we need to show $\delta f(\w_{t+1}) - \delta f(\w_t) \leq -\rho \delta f(\w_t)$.
\begin{align}
& \left[ L^2 \eta^2 (1+\beta) - \eta \mu  + \frac{2LS\alpha}{n} \right] \delta f(\w_t) \stackrel{!}\leq -c\mu \eta \delta f(\w_t) \nonumber \\
& \stackrel{\times 1/\mu \eta L}\Longrightarrow \left[ \frac{L}{2\mu} (1+\beta) \eta - \frac1L \right] + \frac{2S\alpha}{n\eta\mu} \leq \frac{-c}{L} \nonumber \\
& \Longrightarrow \frac{L}{2\mu} (1+\beta) \eta \leq \frac1L - \frac{2S\alpha}{n\eta\mu} - \frac{c}{L} \nonumber \\
& \stackrel{S:=\eta n S'}\Longrightarrow \frac{L}{2\mu} (1+\beta) \eta \leq \frac1L - \frac{2S'\alpha}{\mu} - \frac{c}{L}
\end{align}

Note that if $S'=\frac{\mu}{L}$ then $\eta \leq O(\frac{\mu}{L^2})$.\\


We now consider the term in the second rectangular bracket. We need
\begin{align}
& \left[ \frac{L}{2} \eta^2 (1+\beta^{-1}) - \frac{S\alpha}{n} \right] \stackrel{!}\leq - \rho S\alpha \nonumber \\
& \stackrel{\times 1/S}\Longrightarrow \left[ \frac{L}{2S} \eta^2 (1+\beta^{-1}) - \frac{\alpha}{n} \right] \leq - c \eta \mu \alpha \nonumber \\
& \stackrel{S:=\eta n S'}\Longrightarrow \frac{1}{n} \left[ \frac{L}{2S'} \eta (1+\beta^{-1}) - \alpha \right] \leq - c \eta \mu \alpha \nonumber \\
& \stackrel{\times n/\eta}\Longrightarrow \frac{L}{2S'} (1+\beta^{-1}) - \frac{\alpha}{\eta} \leq - c n \mu \alpha \nonumber \\
& \Longrightarrow \frac{\alpha}{\eta} \geq c n \mu \alpha + \frac{L}{2S'} (1+\beta^{-1}) \nonumber \\
& \Longrightarrow \eta \leq \frac{\alpha}{c n \mu \alpha + \frac{L}{2S'} (1+\beta^{-1})}
\end{align}

%Note that if $S'=\frac{\mu}{L}$ then $\eta \leq O(\frac{\mu}{L^2})$.
%If $S'=\mu$ then $\eta \leq O(\frac{\mu}{L})$.\\

With $S'=\frac{\mu}{L}$, $\beta=1$ we get
\begin{align}
\eta &\leq \min \left\{ 
\frac{\mu(1 - c - 2\alpha)}{L^2},
\frac{\alpha}{c n \mu \alpha + \frac{L^2}{\mu}} \right\} \nonumber \\
\end{align}

\end{proof}





\comment{
\vspace{1cm}
\paragraph{Old stuff}

Using $\eta = \frac1L$, the first term becomes:
$$\left[ \frac{L}{2} \eta^2 (1+\beta) - \eta \right] = \left[ \frac{1}{2L} (1+\beta) - \frac1L \right] = \left[ \frac{\beta - 1}{2L} \right] \stackrel{!}\leq -\frac{a}{L} \Longrightarrow \beta \leq -2a + 1 -4 \alpha$$

We then use strong-convexity to show
\begin{align}
\left[ \frac{L}{2} \eta^2 (1+\beta) - \eta \right] \sqnorm{\nabla f(\w_t)} + \frac{2LS \alpha}{n} \delta f(\w_t)
&\leq \left(-\frac{a \mu}{L} + \frac{2LS \alpha}{n} \right) \delta f(\w_t) \stackrel{!}\leq - c \mu \frac{1}{L}
\end{align}

Second term $\left[ \frac{L}{2} \eta^2 (1+\beta^{-1}) - \frac{S\alpha}{n} \right] \leq - \rho S\alpha$

Using $S = \frac{\eta n}{L}$ yields:
\begin{align}
& \;\;\;\;\; \left[ \frac{L}{2} \eta^2 (1+\beta^{-1}) - \frac{\alpha \eta}{L} \right] \leq - \rho S\alpha = -c \eta^2 \mu \alpha \frac{n}{L} \nonumber \\
& \Longrightarrow \left[ \frac{L}{2} (1+\beta^{-1}) - \frac{\alpha}{L\eta} \right] \leq -c \alpha K, \;\;\;\; K := \frac{n\mu}{L} \nonumber \\
& \Longrightarrow  - \frac{\alpha}{L\eta} \leq -c \alpha K - \frac{L}{2} (1+\beta^{-1}) \nonumber \\
%& \Longrightarrow  \frac{\alpha}{L\eta} \geq c \alpha K - \frac{L}{2} (1+\beta^{-1}) \nonumber \\
& \Longrightarrow  \eta \leq \frac{\alpha}{L(c \alpha K - \frac{L}{2} (1+\beta^{-1}))} = \frac{\alpha}{c \alpha n \mu - \frac{L^2}{2} (1+\beta^{-1})}
\end{align}
}

\comment{
\begin{align}
\delta f(\w_{t+1})
&\leq \delta f(\w_{t}) - \eta \sqnorm{\nabla f(\w_t)} + \frac{L}{2} \eta^2 ((1+\beta) \E \sqnorm{\nabla f_i(\w_t) - \nabla f_i(\wstar)} \nonumber \\
&+ (1+\beta^{-1}) \E \sqnorm{\alpha_i - \nabla f_i(\wstar)}) \nonumber \\
&\leq \delta f(\w_{t}) - \eta \sqnorm{\nabla f(\w_t)} + \frac{L^2}{2} \eta^2 (1+\beta) \delta f(\w_{t}) \nonumber \\
&+ \frac{L}{2} \eta^2 (1+\beta^{-1}) \E \sqnorm{\alpha_i - \nabla f_i(\wstar)} \nonumber
\end{align}

Recall $\E \sqnorm{\alpha_i - \nabla f_i(\wstar)} \leq \Hbar$. We define the following Lyapnunov function $\L(\w, H) := \delta f(\w_{t}) + S\alpha \Hbar$.

We write $\Delta := \L(\w^+, H) - \L(\w, H)$. We get
\begin{align}
\Delta &\leq - \eta \sqnorm{\nabla f(\w_t)} + \frac{L^2}{2} \eta^2 (1+\beta) \delta f(\w_{t}) + \frac{L}{2} \eta^2 (1+\beta^{-1}) \E \sqnorm{\alpha_i - \nabla f_i(\wstar)} \nonumber \\
&+ S\alpha \left( - \frac{1}{n} \Hbar + \frac{2L}{n} \delta f(\w_t) \right) \nonumber \\
&= - \eta \sqnorm{\nabla f(\w_t)} + \frac{L^2}{2} \eta^2 (1+\beta) \delta f(\w_{t}) + \left( \frac{L}{2} \eta^2 (1+\beta^{-1}) - \frac{S\alpha}{n} \right) \Hbar + \frac{2LS \alpha}{n} \delta f(\w_t)
\end{align}

Group the first two terms:
\begin{align}
- \eta \sqnorm{\nabla f(\w_t)} + \frac{L^2}{2} \eta^2 (1+\beta) \delta f(\w_{t}) \leq
\left( \frac{L^2}{2} \eta^2 (1+\beta) - \eta \mu \right) \delta f(\w_{t})
\end{align}

Condition on $\rho$ is too restrictive, need to keep the variance terms together.
}

{\small
\bibliographystyle{splncs}
\bibliography{sgd}
}

%%%%%%%%%%%%%%%%%%%%%%%%%%%%%%%%%%%%%%%%%%%%%%%%%%%%
% OLD STUFF
\comment{
\paragraph{Option 1} Start with bound on iterates:

\begin{align}
\sqnorm{\w_{t+1} - \w^*} &= \sqnorm{\w_t - \eta \nabla f(\w_t) - \w^*} \nonumber \\
&= \sqnorm{\w_t - \w^*} - 2 \eta (\w_t - \w^*)^T \nabla f(\w_t) + \eta^2 \sqnorm{\nabla f(\w_t)} \nonumber \\
&\leq (1 - \eta\mu) \sqnorm{\w_t - \w^*} - 2 \eta (f(\w_t) - f(\wstar)) + 2 \eta^2 L (f(\w_t) - f(\wstar)) \nonumber \\
&= (1 - \eta\mu) \sqnorm{\w_t - \w^*} - 2 \eta (1 - \eta L) (f(\w_t) - f(\wstar))
\end{align}

Using strong-convexity and Lipschitz:
\begin{align}
\frac2L (f(\w_{t+1}) - f(\wstar))
&\leq (1 - \eta\mu) \sqnorm{\w_t - \w^*} - 2 \eta (1 - \eta L) (f(\w_t) - f(\wstar)) \nonumber \\
&\leq \frac{2(1 - \eta\mu)}{\mu} (f(\w_t) - f(\w^*)) - 2 \eta (1 - \eta L) (f(\w_t) - f(\wstar)) \nonumber \\
&= \left( \frac{2(1 - \eta\mu)}{\mu} - 2 \eta (1 - \eta L) \right) (f(\w_t) - f(\w^*))
\end{align}

We thus get:
\begin{align}
(f(\w_{t+1}) - f(\wstar))
&\leq L \left( \frac{(1 - \eta\mu)}{\mu} - \eta (1 - \eta L) \right) (f(\w_t) - f(\w^*))
\end{align}
Need $\rho := L \left( \frac{(1 - \eta\mu)}{\mu} - \eta (1 - \eta L) \right) < 1$...


\paragraph{Gradient Descent}
Use Taylor expansion and upper bound $L$ on the Hessian

Our starting point is the basic inequality
\begin{align}
f(\w_{t+1}) & = f(\w_t - \eta \nabla f(\w_t)) \nonumber \\
&\leq f(\w_{t}) - \eta \langle \nabla f(\w_t), \nabla f(\w_t) \rangle + \frac{L}{2} \eta^2 \sqnorm{\nabla f(\w_t)} \nonumber \\
%&\leq f(\w_{t}) - \eta \left(\mu + \frac{L^2}{2} \eta \right) (f(\w_t) - f(\wstar))
\label{eq:basic_eq}
\end{align}

Plug-in $\eta=\frac1L$ and subtract $f(\wstar)$ on both sides,
\begin{align}
f(\w_{t+1}) - f(\wstar)
&\leq (f(\w_{t}) - f(\wstar)) - \eta \sqnorm{\nabla f(\w_t)} + \frac{L}{2} \eta^2 \sqnorm{\nabla f(\w_t)} \nonumber \\
&= (f(\w_{t}) - f(\wstar)) - \frac{1}{2L} \sqnorm{\nabla f(\w_t)} \nonumber \\
&\leq (f(\w_{t}) - f(\wstar)) - \frac{\mu}{L} (f(\w_{t}) - f(\wstar)) \nonumber \\
&= (f(\w_{t}) - f(\wstar)) (1 - \frac{\mu}{L})
\label{eq:basic_eq}
\end{align}
}

\end{document}
